A boring example. Anyway I can get rid of the axiom?

examples/locks/Locks.hs
@@ -1,0 +1,15 @@
+module Locks where
+
+import           Control.Concurrent.MVar
+
+example :: IO ()
+example = do
+  m <- newMVar 42
+  x <- takeMVar m
+  return ()
+
+deadlock :: IO ()
+deadlock = do
+  m <- newEmptyMVar :: IO (MVar Int)
+  x <- takeMVar m
+  return ()
