base-thy/Control/Concurrency/Interp.v
@@ -1,16 +1,17 @@
 Require Import GHC.MVar.
 Require Import Control.Concurrent.MVar.
+Require Import GHC.Num.
 
 Require Import Streams Arith.
 
-Open Scope nat_scope.
+Open Scope N_scope.
 
 Record heap :=
-  { max_loc : nat;
-    content : nat -> option nat }.
+  { max_loc : Word;
+    content : Word -> option Word }.
 
 Definition empty_heap :=
-  {| max_loc := 0;
+  {| max_loc := #0;
      content := fun _ => None |}.
 
 Definition prog := IO unit.
@@ -35,7 +36,7 @@ Next Obligation.
            |}).
   - destruct m.
     destruct (content h loc) eqn:Hcontent.
-    + destruct (@decode A _ n) eqn:Hdecode.
+    + destruct (@decode A _ w) eqn:Hdecode.
       * right. destruct h.
         exact (k a,
                {| max_loc := max_loc0;
@@ -45,7 +46,7 @@ Next Obligation.
     + left. exact Blocked.
   - destruct m.
     destruct (content h loc) eqn:Hcontent.
-    + destruct (@decode A _ n) eqn:Hdecode.
+    + destruct (@decode A _ w) eqn:Hdecode.
       * right. exact (k a, h).
       * left. exact Unexpected.
     + left. exact Blocked.
@@ -59,7 +60,7 @@ Next Obligation.
              |}).
   - destruct m.
     destruct (content h loc) eqn:Hcontent.
-    + destruct (@decode A _ n) eqn:Hdecode.
+    + destruct (@decode A _ w) eqn:Hdecode.
       * right. destruct h.
         exact (k (Some a),
                {| max_loc := max_loc0;
@@ -69,7 +70,7 @@ Next Obligation.
     + right. exact (k None, h).
   - destruct m.
     destruct (content h loc) eqn:Hcontent.
-    + destruct (@decode A _ n) eqn:Hdecode.
+    + destruct (@decode A _ w) eqn:Hdecode.
       * right. exact (k (Some a), h).
       * left. exact Unexpected.
     + right. exact (k None, h).
@@ -95,3 +96,28 @@ Inductive safe_single_prog_on_heap (p : prog) (h : heap) : Prop :=
 
 Definition safe_single_prog (p : prog) : Prop :=
   safe_single_prog_on_heap p empty_heap.
+
+Inductive deadlock_single_prog_on_heap (p : prog) (h : heap) : Prop :=
+| DeadlockBlocked (_ : interp p h = inl Blocked)
+| DeadlockRunning : forall p' h', interp p h = inr (p', h') ->
+                             deadlock_single_prog_on_heap p' h' ->
+                             deadlock_single_prog_on_heap p h.
+
+Definition deadlock_single_prog (p : prog) : Prop :=
+  deadlock_single_prog_on_heap p empty_heap.
+
+Lemma deadlock_unsafe' : forall p h,
+    deadlock_single_prog_on_heap p h -> ~ safe_single_prog_on_heap p h.
+Proof.
+  induction 1. 
+  - inversion 1; subst; rewrite H1 in H; discriminate.
+  - inversion 1; rewrite H2 in H.
+    + discriminate.
+    + inversion H; subst. contradiction.
+Qed.
+
+Lemma deadlock_unsafe : forall p,
+    deadlock_single_prog p -> ~ safe_single_prog p.
+Proof.
+  intro p. apply deadlock_unsafe'.
+Qed.
