examples/locks/Proofs.v
@@ -1,0 +1,33 @@
+Require Import GHC.Num.
+Require Import GHC.MVar.
+Require Import Control.Concurrent.MVar.
+Require Import Proofs.Control.Concurrency.Interp.
+
+Require Import Locks.
+
+Axiom decode_encode_word : forall (w : Word),
+    decode (encode w) = Some w.
+
+Ltac forward := first
+                  [apply SafeFinished; reflexivity |
+                   eapply SafeRunning; [try reflexivity |] |
+                   apply DeadlockBlocked; reflexivity |
+                   eapply DeadlockRunning; [try reflexivity |]
+                  ].
+                   
+Theorem example_prog_safe : safe_single_prog example.
+Proof.
+  do 3 forward.
+  - simpl; rewrite decode_encode_word. reflexivity.
+  - forward.
+Qed.
+
+Lemma deadlock_prog_deadlock : deadlock_single_prog deadlock.
+Proof.
+  do 2 forward.
+Qed.
+
+Theorem deadlock_prog_unsafe : ~ safe_single_prog deadlock.
+Proof.
+  apply deadlock_unsafe. apply deadlock_prog_deadlock.
+Qed.
